Final of 2015 Fall Semester

Adv Operating Systems/Project4/tests/test.cpp
@@ -1,0 +1,144 @@
+#include "test.h"
+#include <map>
+#include <string>
+#include <string.h>
+#include <sys/stat.h>
+#include <unistd.h>
+#include <sys/types.h>
+#include <vector>
+#include <assert.h>
+#include <stdlib.h>
+#include <iostream>
+
+using namespace std;
+int main() {
+    //FILE *fp = fopen("/Users/bianshujun/Desktop/test.log", "r");
+    FILE * fp = fopen("/Users/bianshujun/Desktop/a.txt", "r+");
+    if (fp == NULL) {
+        cerr << "file error" << endl;
+        exit(1);
+    }
+ 
+    fseek(fp, 1, SEEK_SET);
+    fwrite("ggg", 1, 3, fp);
+ 
+    fclose(fp);
+ 
+    return 0;
+/*
+    std::vector<region_t *> region_list;
+    for (int i = 0; i < 3; i++) {
+
+        segment_t* tempSeg = new segment_t();
+        tempSeg->seg_name = "data";
+        tempSeg->seg_size = 3 * (i + 1);
+        char* data = new char[10];
+        sprintf(data, "prae_%d_suff", i);
+        tempSeg->data = data;
+
+        region_t* tempRegion = new region_t();
+        tempRegion->segment = tempSeg;
+        tempRegion->offset = i + 3;
+        tempRegion->size = 4;
+        std::string tempStr = "String";
+        tempStr += i;
+        tempRegion->undo_data = &tempStr;
+
+        region_list.push_back(tempRegion);
+    }
+
+    // for (int i = 0; i < 3; i++) {
+    //     std::cout << (char*)region_list[i]->segment->data << std::endl;
+    // }
+
+
+    trans_header_t txheader;
+    trans_end_t txender;
+    txheader.recordnum = 0;
+    txheader.length = sizeof(trans_header_t) + sizeof(trans_end_t);
+    txheader.tid = 79;
+
+    for (std::vector<region_t *>::iterator it = region_list.begin(); it!=region_list.end(); it++)
+    {
+        txheader.recordnum++;
+        txheader.length += (sizeof(int)+strlen((*it)->segment->seg_name)+sizeof(int)*2+(*it)->size);
+    }
+    
+    txender.recordnum = txheader.recordnum;
+    txender.length = txheader. length;        
+    txender.tid = 79;
+    
+    fwrite(&txheader, 1, sizeof(trans_header_t), fp);
+    
+    for (std::vector<region_t *>::iterator it = region_list.begin(); it!=region_list.end(); it++)
+    {
+        char buf[256];
+        int len;
+        len = strlen((*it)->segment->seg_name);
+        memcpy(buf, (char*)&len, sizeof(int));
+        memcpy(buf + sizeof(int), (*it)->segment->seg_name, len);
+        memcpy(buf + sizeof(int)+len, &((*it)->offset), sizeof(int));
+        memcpy(buf + sizeof(int)+len+ sizeof(int), &((*it)->size), sizeof(int));
+        fwrite(buf, 1, sizeof(int)+len+ sizeof(int)*2, fp);
+        fwrite((char *)(*it)->segment->data + (*it)->offset, 1, (*it)->size, fp);
+    }
+    fwrite(&txender, 1, sizeof(trans_end_t), fp);
+    fclose(fp);
+*/
+    //fp = fopen("/Users/bianshujun/Desktop/test.log", "r");
+/*
+    std::vector<logrecordheader_t *> record_list;
+
+    while(!feof(fp))
+    {
+       trans_header_t r_txheader;
+       fread(&r_txheader, sizeof(trans_header_t), 1, fp);
+    std::cout<< r_txheader.recordnum << std::endl;
+
+       for (int i = 0; i < r_txheader.recordnum; i++) {
+            //std::cout << i << std::endl;
+        logrecordheader_t* record = new logrecordheader_t();
+        int segnameLen;
+        fread(&segnameLen, sizeof(int), 1, fp);
+        fread(&(record->segmentname), segnameLen, 1, fp);
+            // std::cout << (char*)record->segmentname << std::endl;
+
+        fread(&(record->region_offset), sizeof(int), 1, fp);
+        fread(&(record->region_size), sizeof(int), 1, fp);
+            // std::cout << record->region_offset << "   " << record->region_size << std::endl;
+
+        record->data = (void*)malloc(record->region_size);
+        fread(record->data, record->region_size, 1, fp);
+        // std::cout << (char*)record->data << std::endl;
+        record_list.push_back(record);
+        }
+
+    trans_end_t r_txender;
+    fread(&r_txender, sizeof(trans_header_t), 1, fp);
+    if (r_txender.tid != r_txheader.tid || 
+        r_txender.length != r_txheader.length ||
+        r_txender.recordnum != r_txheader.recordnum) {
+        std::cout << record_list.size() << std::endl;
+        for (std::vector<logrecordheader_t *>::iterator it = record_list.end() - r_txheader.recordnum;
+            it != record_list.end(); it++) {
+            free((*it)->data);
+            free(*it);            
+            //delete a pointer in struct?
+        }
+        record_list.erase(record_list.end() - r_txheader.recordnum, record_list.end());
+    }
+
+    r_txheader.recordnum = 0;
+    r_txender.recordnum = 0;
+}
+fclose(fp);
+*/
+//std::cout << record_list[0]->segmentname << std::endl;
+// std::cout << record_list.size() << std::endl;
+
+    //std::string fileName = record_list[0]->segmentname;
+
+
+system( "read -n 1 -s -p \"Press any key to continue...\"" );
+
+}
