Programming Languages/Final.v
@@ -1,0 +1,257 @@
+Require Export Hoare.
+Require Export Imp.
+Require Export Types.
+Require Export Smallstep.
+
+(*Imperative Summation*)
+(*
+  {{ X = n }}
+  I ::= 0;;
+  Z ::= 0;;
+  WHILE  I  <>  X+1  DO
+    I ::= I + 1;;
+    Z ::= Z + X
+  END;;
+  Y ::= 0;;
+  WHILE Z<>0 Do
+    Y ::= Y + 1;;
+    Z ::= Z - 2
+  END
+  {{2 * Y = n * (S n)}}
+
+  {{X = n}} ->>
+  {{0 = 0 * n /\ X = n}}
+  I ::=0 ;;
+  {{0 = I * n /\ X = n}}
+  Z ::= 0;;
+  {{Z = I * n /\ X = n}}
+
+  WHILE I <> X + 1 DO
+    {{Z = I * n /\ X = n /\ I <> X + 1}} ->>
+    {{Z + X = (I + 1) * n /\ X = n}}
+    I ::= I + 1;;
+    {{Z + X = I * n /\ X = n}}
+    Z ::= Z + X
+    {{Z = I * n /\ X = n}}
+  END
+
+  {{Z = I * n /\ X = n /\ I = X + 1}} ->>
+  {{Z = n * (n + 1)}} ->>
+  {{2 * 0 + Z = n * (n + 1)}}
+  Y ::= 0;;
+  {{2 * Y + Z = n * (n + 1)}}
+  WHILE Z <> 0 DO
+    {{2 * Y + Z = n *(n + 1) /\ Z <> 0}} ->>
+    {{2 * (Y + 1) + (Z - 2) = n *(n + 1)}}
+    Y ::= Y + 1;;
+    {{2 * Y + (Z - 2) = n * (n + 1)}}
+    Z ::= Z - 2
+    {{2 * Y + Z = n * (n + 1)}}
+  END
+  
+  {{2 * Y + Z = n * (n + 1) /\ (Z = 0)}} ->>
+  {{2 * Y = n * (n + 1)}} ->>
+  {{2 * Y = n * (S n)}}
+*)
+
+(*Types*)
+Inductive tm : Type :=
+  | ttrue : tm
+  | tfalse : tm
+  | tif : tm -> tm -> tm -> tm
+  | tzero : tm
+  | tplus : tm-> tm -> tm
+  | tsucc : tm -> tm
+  | tpred : tm -> tm
+  | tiszero : tm -> tm.
+
+
+Reserved Notation "t1 '==>' t2" (at level 40).
+
+Inductive step : tm -> tm -> Prop :=
+  | ST_IfTrue : forall t1 t2,
+      (tif ttrue t1 t2) ==> t1
+  | ST_IfFalse : forall t1 t2,
+      (tif tfalse t1 t2) ==> t2
+  | ST_If : forall t1 t1' t2 t3,
+      t1 ==> t1' ->
+      (tif t1 t2 t3) ==> (tif t1' t2 t3)
+  | ST_Succ : forall t1 t1',
+      t1 ==> t1' ->
+      (tsucc t1) ==> (tsucc t1')
+  | ST_PlusZero : forall t1,
+    nvalue t1 ->
+    tplus tzero t1 ==> t1
+  |ST_PlusSucc : forall t1 t1',
+    nvalue t1 -> nvalue t1' ->
+    tplus (tsucc t1) t1' ==> tplus t1 (tsucc t1')
+  | ST_Plus : forall t0 t1 t2,
+    t0 ==> t1 ->
+    tplus t2 t0 ==> tplus t2 t1
+ | ST_Plus2: forall t0 t1 t2,
+    t0 ==> t1 ->
+    (tplus t0 t2) ==> (tplus t1 t2)
+  | ST_PredZero :
+      (tpred tzero) ==> tzero
+  | ST_PredSucc : forall t1,
+      nvalue t1 ->
+      (tpred (tsucc t1)) ==> t1
+  | ST_Pred : forall t1 t1',
+      t1 ==> t1' ->
+      (tpred t1) ==> (tpred t1')
+  | ST_IszeroZero :
+      (tiszero tzero) ==> ttrue
+  | ST_IszeroSucc : forall t1,
+       nvalue t1 ->
+      (tiszero (tsucc t1)) ==> tfalse
+  | ST_Iszero : forall t1 t1',
+      t1 ==> t1' ->
+      (tiszero t1) ==> (tiszero t1')
+
+where "t1 '==>' t2" := (step t1 t2).
+
+
+Inductive ty : Type := 
+  | TBool : ty
+  | TNat : ty.
+  
+Reserved Notation "'|-' t '\in' T" (at level 40).
+
+Inductive has_type : tm -> ty -> Prop :=
+  | T_True : 
+       |- ttrue \in TBool
+  | T_False : 
+       |- tfalse \in TBool
+  | T_If : forall t1 t2 t3 T,
+       |- t1 \in TBool ->
+       |- t2 \in T ->
+       |- t3 \in T ->
+       |- tif t1 t2 t3 \in T
+  | T_Zero : 
+       |- tzero \in TNat
+  | T_Succ : forall t1,
+       |- t1 \in TNat ->
+       |- tsucc t1 \in TNat
+  | T_Pred : forall t1,
+       |- t1 \in TNat ->
+       |- tpred t1 \in TNat
+  | T_Iszero : forall t1,
+       |- t1 \in TNat ->
+       |- tiszero t1 \in TBool
+  | T_Plus : forall t0 t1,
+       |- t0 \in TNat ->
+       |- t1 \in TNat ->
+       |- tplus t0 t1 \in TNat
+
+where "'|-' t '\in' T" := (has_type t T).
+
+
+Hint Constructors has_type.
+
+Theorem progress : forall t T,
+  |- t \in T ->
+  value t \/ exists t', t ==> t'.
+
+(** **** Exercise: 3 stars (finish_progress)  *)
+(** Complete the formal proof of the [progress] property.  (Make sure
+    you understand the informal proof fragment in the following
+    exercise before starting -- this will save you a lot of time.) *)
+
+Proof with auto.
+  intros t T HT.
+  has_type_cases (induction HT) Case...
+  (* The cases that were obviously values, like T_True and
+     T_False, were eliminated immediately by auto *)
+  Case "T_If".
+    right. inversion IHHT1; clear IHHT1.
+    SCase "t1 is a value".
+    apply (bool_canonical t1 HT1) in H.
+    inversion H; subst; clear H.
+      exists t2...
+      exists t3...
+    SCase "t1 can take a step".
+      inversion H as [t1' H1].
+      exists (tif t1' t2 t3)...
+  Case "T_Succ". inversion IHHT.
+    SCase "t1 is a value". inversion H; clear H.
+      SSCase "t1 is a bvalue". solve by inversion 2.
+      SSCase "t1 is a nvalue". left...
+    SCase "t1 can take a step".
+     right. inversion H as [t' H']. exists (tsucc t')...
+  Case "T_Pred". inversion IHHT.
+    SCase "t1 is a value". inversion H; clear H.
+      SSCase "t1 is a bvalue". solve by inversion 2.
+      SSCase "t1 is a nvalue". right. inversion H0; eauto.
+    SCase "t1 can take a step".
+      right. inversion H as [t' H']. exists (tpred t')...
+  Case "T_Iszero". right. inversion IHHT.
+    SCase "t1 is a value". inversion H; clear H.
+      SSCase "t1 is a bvalue". solve by inversion 2.
+      SSCase "t1 is a nvalue". inversion H0.
+        SSSCase "t1 is tzero". exists ttrue...
+        SSSCase "t1 is tsucc t". exists tfalse...
+    SCase "t1 can take a step".
+      inversion H as [t' H']. exists (tiszero t')...
+  Case "T_Plus".
+      inversion IHHT1.
+      SCase "t0 is a value". inversion H; clear H.
+        SSCase "t0 is a bvalue". solve by inversion 2.
+        SSCase "t0 is a nvalue". inversion H0.
+          SSSCase "t0 is tzero". 
+            inversion IHHT2.
+            SSSSCase "t1 is a value". inversion H1; clear H1.
+              SSSSSCase "t1 is a bvalue". solve by inversion 2.
+              SSSSSCase "t1 is a nvalue". inversion H2.
+                SSSSSSCase "t1 is tzero". right. exists tzero...
+                SSSSSSCase "t1 is tsucc t". right. rewrite H3. exists t1...
+           SSSSCase "t1 can take a step".
+             inversion H1 as [t' H1']. right. exists (tplus tzero t')...
+        SSSCase "t0 is not tzero". right.
+          inversion IHHT2.
+          SSSSCase "t1 is a value". inversion H2; clear H1. assert (nvalue t1).
+          apply nat_canonical. assumption. assumption.
+          exists (tplus t (tsucc t1)). constructor. assumption. assumption.
+          exists (tplus t (tsucc t1)). constructor. assumption. assumption.
+          SSSSCase "t1 can take a step".
+            inversion H2 as [t' H1']. exists (tplus (tsucc t) t')...
+   SCase "t1 can take a step". right. 
+            inversion H as [t' H']. exists (tplus t' t1)...
+Qed.
+Theorem preservation : forall t t' T,
+  |- t \in T ->
+  t ==> t' ->
+  |- t' \in T.
+
+(** **** Exercise: 2 stars (finish_preservation)  *)
+(** Complete the formal proof of the [preservation] property.  (Again,
+    make sure you understand the informal proof fragment in the
+    following exercise first.) *)
+
+Proof with auto.
+  intros t t' T HT HE.
+  generalize dependent t'.
+  has_type_cases (induction HT) Case; 
+         (* every case needs to introduce a couple of things *)
+         intros t' HE; 
+         (* and we can deal with several impossible
+            cases all at once *)
+         try (solve by inversion).
+    Case "T_If". inversion HE; subst; clear HE.
+      SCase "ST_IFTrue". assumption.
+      SCase "ST_IfFalse". assumption.
+      SCase "ST_If". apply T_If; try assumption.
+        apply IHHT1; assumption.
+       Case "T_Succ".
+      inversion HE; subst...
+    Case "T_Pred".
+      inversion HE; subst...
+      assert (forall t, nvalue t -> has_type t TNat).
+        intros. induction H. constructor.
+        constructor. apply IHnvalue.
+      apply H...
+    Case "T_Iszero".
+      inversion HE; subst...
+    Case "T_Plus".
+      inversion HE; subst... constructor. inversion HT1; subst...
+      constructor. assumption.
+Qed.
