Programming Languages/Resource/sf/Hoare.v
@@ -1524,12 +1524,15 @@ Notation "{{ P }}  c  {{ Q }}" := (hoare_triple P c Q)
     [havoc_pre] and prove that the resulting rule is correct. *)
 
 Definition havoc_pre (X : id) (Q : Assertion) : Assertion :=
-(* FILL IN HERE *) admit.
+  fun st => forall n, Q (update st X n).
 
 Theorem hoare_havoc : forall (Q : Assertion) (X : id),
   {{ havoc_pre X Q }} HAVOC X {{ Q }}.
 Proof.
-  (* FILL IN HERE *) Admitted.
+  intros Q X st st' H1 H2.
+  inversion H1. subst.
+  unfold havoc_pre in H2. apply H2.
+Qed.
 
 End Himp.
 (** [] *)
